refactor

theories/imp_to_asm.v
@@ -8,155 +8,6 @@ Require Import refframe.imp.
 Require Import refframe.asm.
 Require Import refframe.itree.
 
-(*** [mod_seq_map] *)
-Inductive mod_seq_map_state {EV1 : Type} :=
-| SMProg
-| SMProgRecv (e : EV1)
-| SMFilter
-| SMFilterRecv (e : EV1)
-.
-Arguments mod_seq_map_state _ : clear implicits.
-
-Inductive mod_seq_map_filter {EV1 EV2} :
-  mod_seq_map_state EV1 → (seq_product_event EV1 (EV1 + EV2)) → option EV2 → mod_seq_map_state EV1 → Prop :=
-| SeqMapToFilter e:
-  mod_seq_map_filter SMProg (SPELeft e SPRight) None (SMFilterRecv e)
-| SeqMapFilterRecv e:
-  mod_seq_map_filter (SMFilterRecv e) (SPERight (inl e) SPRight) None SMFilter
-| SeqMapFilterOut e:
-  mod_seq_map_filter SMFilter (SPERight (inr e) SPRight) (Some e) SMFilter
-| SeqMapFilterToProg e:
-  mod_seq_map_filter SMFilter (SPERight (inl e) SPLeft) (None) (SMProgRecv e)
-| SeqMapProgRecv e:
-  mod_seq_map_filter (SMProgRecv e) (SPELeft e SPLeft) None SMProg
-.
-
-Definition mod_seq_map {EV1 EV2} (m : module EV1) (f : module (EV1 + EV2)) : module EV2 :=
-  mod_map (mod_seq_product m f) mod_seq_map_filter.
-Global Hint Transparent mod_seq_map : tstep.
-
-Lemma mod_seq_map_nil_l {EV1 EV2} m (f : module (EV1 + EV2)) σ Pσ Pσf σf κs σm:
-  σ ~{ m, tnil }~>ₜ Pσ →
-  (∀ σ', Pσ σ' → (SPLeft, σ', σf, σm) ~{ mod_seq_map m f, κs }~>ₜ Pσf) →
-  (SPLeft, σ, σf, σm) ~{ mod_seq_map m f, κs }~>ₜ Pσf.
-Proof.
-  move => Hσ Hcont.
-  apply: mod_map_nil.
-  - by apply: seq_product_nil_l.
-  - move => [[??]?] /=. naive_solver.
-Qed.
-
-Lemma mod_seq_map_nil_r {EV1 EV2} m (f : module (EV1 + EV2)) σ Pσ Pσf σf κs σm:
-  σf ~{ f, tnil }~>ₜ Pσ →
-  (∀ σ', Pσ σ' → (SPRight, σ, σ', σm) ~{ mod_seq_map m f, κs }~>ₜ Pσf) →
-  (SPRight, σ, σf, σm) ~{ mod_seq_map m f, κs }~>ₜ Pσf.
-Proof.
-  move => Hσ Hcont.
-  apply: mod_map_nil.
-  - by apply: seq_product_nil_r.
-  - move => [[??]?] /=. naive_solver.
-Qed.
-
-Lemma mod_seq_map_step_filter_i {EV1 EV2} m (f : module (EV1 + EV2)) σ σf P `{!TStepI f σf P} :
-  TStepI (mod_seq_map m f) (SPRight, σ, σf, SMFilter) (λ G, P (λ b κ P',
-    match κ with
-    | None => G b None (λ G', P' (λ x, G' (SPRight, σ, x, SMFilter)))
-    | Some (inr e) => G b (Some e) (λ G', P' (λ x, G' (SPRight, σ, x, SMFilter)))
-    | Some (inl e) => G b None (λ G', P' (λ x, G' (SPLeft, σ, x, SMProgRecv e)))
-    end)).
-Proof.
-  constructor => G /tstepi_proof?. clear TStepI0.
-  (* Set Typeclasses Debug. *)
-  (* tstep_i.  *)
-  (* apply: steps_impl_mono; [done|]. *)
-  (* move => ? κ ?/= [?[?[?[??]]]] ?? κ' ??. *)
-  (* destruct κ as [[e|e]|]; simplify_eq/=. *)
-  apply: (steps_impl_submodule _ (mod_seq_map _ _) (λ x, (SPRight, σ, x, SMFilter))); [done| |].
-  - move => /= ?? [?[? [? [? HG']]]]. eexists _, _. split_and!; [done..|] => /= ? /HG'. naive_solver.
-  - move => /= ??? Hs. invert_all' @filter_step; simplify_eq. invert_all' @m_step; simplify_eq/=.
-    case_match; simplify_eq. all: eexists _, _; split; [done|] => /=; split_and! => /= *; destruct_all?.
-    + eexists _, _. split_and!; [done..|]. move => /= ? /H2 [?[??]]. eexists (_, _, _, _). naive_solver.
-    + naive_solver.
-    + admit.
-    + naive_solver.
-Admitted.
-Global Hint Resolve mod_seq_map_step_filter_i | 1 : tstep.
-
-Lemma mod_seq_map_step_filter_recv_i {EV1 EV2} m (f : module (EV1 + EV2)) σ σf P `{!TStepI f σf P} e :
-  TStepI (mod_seq_map m f) (SPRight, σ, σf, SMFilterRecv e) (λ G, P (λ b κ P',
-       if κ is Some e' then inl e = e' → G b None (λ G', P' (λ x, G' (SPRight, σ, x, SMFilter)))
-       else G b None (λ G', P' (λ x, G' (SPRight, σ, x, SMFilterRecv e))))).
-Proof. Admitted.
-Global Hint Resolve mod_seq_map_step_filter_recv_i | 1 : tstep.
-
-Lemma mod_seq_map_step_prog_i {EV1 EV2} m (f : module (EV1 + EV2)) σ σf P `{!TStepI m σ P}:
-  TStepI (mod_seq_map m f) (SPLeft, σ, σf, SMProg) (λ G, P (λ b κ P',
-   G b None (λ G', P' (λ x, if κ is Some e then G' (SPRight, x, σf, SMFilterRecv e)
-                            else G' (SPLeft, x, σf, SMProg))))).
-Proof. Admitted.
-Global Hint Resolve mod_seq_map_step_prog_i | 1 : tstep.
-
-Lemma mod_seq_map_step_prog_recv_i {EV1 EV2} m (f : module (EV1 + EV2)) σ σf P `{!TStepI m σ P} e:
-  TStepI (mod_seq_map m f) (SPLeft, σ, σf, SMProgRecv e) (λ G, P (λ b κ P',
-   if κ is Some e' then e = e' → G b None (λ G', P' (λ x, G' (SPLeft, x, σf, SMProg)))
-                 else G b None (λ G', P' (λ x, G' (SPLeft, x, σf, SMProgRecv e))))).
-Proof. Admitted.
-Global Hint Resolve mod_seq_map_step_prog_recv_i | 1 : tstep.
-
-Lemma mod_seq_map_step_filter_s {EV1 EV2} m (f : module (EV1 + EV2)) σ σf P `{!TStepS f σf P} :
-  TStepS (mod_seq_map m f) (SPRight, σ, σf, SMFilter) (λ G, P (λ κ P',
-    match κ with
-    | None => G None (λ G', P' (λ x, G' (SPRight, σ, x, SMFilter)))
-    | Some (inr e) => G (Some e) (λ G', P' (λ x, G' (SPRight, σ, x, SMFilter)))
-    | Some (inl e) => G None (λ G', P' (λ x, G' (SPLeft, σ, x, SMProgRecv e)))
-    end)).
-Proof.
-  constructor => G /tsteps_proof [κ [? [? HG']]]. clear TStepS0.
-  destruct κ as [[e|e]|]. all: eexists _, _; split; [done|] => G' /= /HG'?; tstep_s.
-  - eexists (Some (inl e)), _. split; [done|]. eexists _, _ => /=. split_and!; [econs|done|done].
-  - eexists (Some (inr e)), _. split; [done|]. eexists _, _ => /=. split_and!; [econs|done|done].
-  - eexists None, _. split; [done|]. eexists _, _ => /=. naive_solver.
-Qed.
-Global Hint Resolve mod_seq_map_step_filter_s | 1 : tstep.
-
-Lemma mod_seq_map_step_filter_recv_s {EV1 EV2} m (f : module (EV1 + EV2)) σ σf P `{!TStepS f σf P} e:
-  TStepS (mod_seq_map m f) (SPRight, σ, σf, SMFilterRecv e) (λ G, P (λ κ P',
-   G None (λ G', if κ is Some e' then inl e = e' ∧ P' (λ x, G' (SPRight, σ, x, SMFilter))
-                 else P' (λ x, G' (SPRight, σ, x, SMFilterRecv e))))).
-Proof.
-  constructor => G /tsteps_proof [κ [? [? HG']]]. eexists _, _. split; [done|].
-  move => ? /=?. clear TStepS0. tstep_s. eexists κ, _. split; [by case_match|].
-  case_match; destruct_all?; simplify_eq; eexists _, _ => /=.
-  - split_and!; [econs|done|]. by apply HG'.
-  - split_and!; [done..|]. by apply HG'.
-Qed.
-Global Hint Resolve mod_seq_map_step_filter_recv_s | 1 : tstep.
-
-Lemma mod_seq_map_step_prog_s {EV1 EV2} m (f : module (EV1 + EV2)) σ σf P `{!TStepS m σ P}:
-  TStepS (mod_seq_map m f) (SPLeft, σ, σf, SMProg) (λ G, P (λ κ P',
-   G None (λ G', P' (λ x, if κ is Some e then G' (SPRight, x, σf, SMFilterRecv e)
-                          else G' (SPLeft, x, σf, SMProg))))).
-Proof.
-  constructor => G /tsteps_proof [κ [? [? HG']]]. eexists _, _. split; [done|].
-  move => ? /=?. clear TStepS0. tstep_s.
-  eexists κ; case_match; eexists _; (split; [done|]); eexists _, _ => /=.
-  - split_and!; [econs|done|naive_solver].
-  - split_and!; [done..|naive_solver].
-Qed.
-Global Hint Resolve mod_seq_map_step_prog_s | 1 : tstep.
-
-Lemma mod_seq_map_step_prog_recv_s {EV1 EV2} m (f : module (EV1 + EV2)) σ σf P `{!TStepS m σ P} e:
-  TStepS (mod_seq_map m f) (SPLeft, σ, σf, SMProgRecv e) (λ G, P (λ κ P',
-   G None (λ G', if κ is Some e' then e = e' ∧ P' (λ x, G' (SPLeft, x, σf, SMProg))
-                 else P' (λ x, G' (SPLeft, x, σf, SMProgRecv e))))).
-Proof.
-  constructor => G /tsteps_proof [κ [? [? HG']]]. eexists _, _. split; [done|].
-  move => ? /=?. clear TStepS0. tstep_s. eexists κ, _. split; [by case_match|].
-  case_match; destruct_all?; simplify_eq; eexists _, _ => /=.
-  - split_and!; [econs|done|]. by apply HG'.
-  - split_and!; [done..|]. by apply HG'.
-Qed.
-Global Hint Resolve mod_seq_map_step_prog_recv_s | 1 : tstep.
 
 (** * imp_to_asm *)
 Definition imp_to_asm_args (ret : Z) (rs : gmap string Z) (vs : list val) : Prop.
@@ -331,7 +182,6 @@ Definition imp_to_asm_combine_inv (m1 m2 : module imp_event)
       ∧ σf1 = SMFilter ∧ σpi1 = SPRight ∧ σpi2 = SPLeft
       ∧ σpi = SPRight
       ∧ ips = IPFRight)).
-Hint Constants Transparent : tstep.
 Ltac solve_imp_to_asm_combine_inv :=
   eexists _, _; split_and!; [naive_solver..| try done; try by econs | naive_solver].
 
@@ -346,6 +196,7 @@ Next Obligation. move => *. setoid_rewrite unfold_forever at 1. by setoid_rewrit
 Global Hint Resolve itree_step_forever_i : tstep.
 
 Axiom ELIM_EUTT : ∀ EV R (t1 t2 : itree EV R), t1 ≈ t2 -> t1 = t2.
+Local Hint Constants Transparent : tstep.
 Local Ltac go :=
       unfold itree_rel; intros; destruct_all?; simplify_eq/=; repeat lazymatch goal with | H : _ ≈ _ |- _ => apply ELIM_EUTT in H; subst end.
 Local Ltac go_i := tstep_i; go.
